Fetch Class for proof context of Instance

coqlspclient/proof_state.py
@@ -231,7 +231,7 @@ class ProofState(object):
         fun = lambda x: x.endswith("(default interpretation)")
         return nots[0][:-25] if fun(nots[0]) else nots[0]
 
-    def __step_context(self):
+    def __step_context(self, step=None):
         def traverse_ast(el):
             if isinstance(el, dict):
                 return [x for v in el.values() for x in traverse_ast(v)]
@@ -261,7 +261,9 @@ class ProofState(object):
 
             return []
 
-        return traverse_ast(self.__current_step.ast.span)
+        if step is None:
+            step = self.__current_step.ast
+        return traverse_ast(step.span)
 
     def __get_last_term(self):
         terms = self.coq_file.terms
@@ -275,6 +277,14 @@ class ProofState(object):
             ):
                 last_term = term
         return last_term
+
+    def __get_instance_context(self):
+        instance_expr = CoqFile.expr(self.__get_last_term().ast)
+        class_id = instance_expr[3]["v"][1]["v"][1]["v"][2][1]
+        class_term = self.__get_term(class_id)
+        class_context = self.__step_context(class_term.ast)
+        not_class = lambda x: not isinstance(x[1], Term) or x[1].text != class_term.text
+        return class_term, list(filter(not_class, class_context))
 
     def __get_program_context(self):
         def traverse_ast(el, keep_id=False):
@@ -360,6 +370,8 @@ class ProofState(object):
         term, statement_context = None, None
         if CoqFile.get_term_type(self.__current_step.ast) == TermType.OBLIGATION:
             term, statement_context = self.__get_program_context()
+        elif CoqFile.get_term_type(self.__current_step.ast) == TermType.INSTANCE:
+            term, statement_context = self.__get_instance_context()
         elif CoqFile.get_term_type(self.__current_step.ast) != TermType.OTHER:
             term = self.__get_last_term()
             statement_context = self.__step_context()
@@ -374,8 +386,7 @@ class ProofState(object):
         def call_context(calls: List[Tuple]):
             context, calls = [], [call[0](*call[1:]) for call in calls]
             [context.append(call) for call in calls if call not in context]
-            context = list(filter(lambda term: term is not None, context))
-            return context
+            return list(filter(lambda term: term is not None, context))
 
         def get_proof_step(step: Tuple[Step, Optional[GoalAnswer], List[Tuple]]):
             return ProofStep(step[0], step[1], call_context(step[2]))
@@ -395,8 +406,8 @@ class ProofState(object):
             raise e
 
         proof_steps = [
-            (term, call_context(context), list(map(get_proof_step, steps)))
-            for term, context, steps in proofs
+            (term, call_context(calls), list(map(get_proof_step, steps)))
+            for term, calls, steps in proofs
         ]
         return list(map(lambda t: ProofTerm(*t), proof_steps))
 
